src/program_proof/pav/history.v
@@ -1,0 +1,18 @@
+From Perennial.program_proof Require Import grove_prelude.
+From Goose.github_com.mit_pdos.pav Require Import kt.
+
+Module HistEntry.
+Record t :=
+  mk {
+    Epoch: w64;
+    HistVal: list w8;
+  }.
+Section defs.
+Context `{!heapGS Σ}.
+Definition own (ptr : loc) (obj : t) : iProp Σ :=
+  ∃ sl_HistVal,
+  "Hptr_Epoch" ∷ ptr ↦[HistEntry :: "Epoch"] #obj.(Epoch) ∗
+  "Hptr_HistVal" ∷ ptr ↦[HistEntry :: "HistVal"] (slice_val sl_HistVal) ∗
+  "#Hsl_HistVal" ∷ own_slice_small sl_HistVal byteT DfracDiscarded obj.(HistVal).
+End defs.
+End HistEntry.
